theories/rule_misc.v
@@ -594,76 +594,153 @@ From HypVeri Require Import RAs.
   (*     (* TODO, seems like we need a lemma: ∀ i, vec1 !!! i = vec2 !!! i -> vec1=vec2 *) *)
   (*         Admitted. *)
 
-  Lemma update_page_table_batch_preserve_current_vm σ (ps: list PID) perm:
-   get_current_vm (update_page_table_batch σ ps perm) = get_current_vm σ.
+  Lemma update_ownership_batch_preserve_current_vm σ (ps: list PID) perm:
+   get_current_vm (update_ownership_batch σ ps perm) = get_current_vm σ.
     Proof.
       rewrite /get_current_vm.
       f_equal.
 Qed.
 
-  Lemma update_page_table_batch_preserve_regs σ (ps: list PID) perm:
-   get_reg_gmap (update_page_table_batch σ ps perm) = get_reg_gmap σ.
+  Lemma update_ownership_batch_preserve_regs σ (ps: list PID) perm:
+   get_reg_gmap (update_ownership_batch σ ps perm) = get_reg_gmap σ.
     Proof.
       rewrite /get_reg_gmap.
       f_equal.
 Qed.
-   Lemma update_page_table_batch_preserve_mem σ (ps: list PID) perm:
-   get_mem (update_page_table_batch σ ps perm) = get_mem σ.
+   Lemma update_ownership_batch_preserve_mem σ (ps: list PID) perm:
+   get_mem (update_ownership_batch σ ps perm) = get_mem σ.
     Proof.
       rewrite /get_mem.
       f_equal.
 Qed.
-   Lemma update_page_table_batch_preserve_tx σ (ps: list PID) perm:
-   get_tx_agree (update_page_table_batch σ ps perm) = get_tx_agree σ.
+   Lemma update_ownership_batch_preserve_tx σ (ps: list PID) perm:
+   get_tx_agree (update_ownership_batch σ ps perm) = get_tx_agree σ.
     Proof.
       rewrite /get_tx_agree.
       f_equal.
 Qed.
-       Lemma update_page_table_batch_preserve_rx1 σ (ps: list PID) perm:
-   get_rx_agree (update_page_table_batch σ ps perm) = get_rx_agree σ.
+       Lemma update_ownership_batch_preserve_rx1 σ (ps: list PID) perm:
+   get_rx_agree (update_ownership_batch σ ps perm) = get_rx_agree σ.
     Proof.
       rewrite /get_rx_agree.
       f_equal.
 Qed.
-   Lemma update_page_table_batch_preserve_rx2 σ (ps: list PID) perm:
-   get_rx_gmap (update_page_table_batch σ ps perm) = get_rx_gmap σ.
+   Lemma update_ownership_batch_preserve_rx2 σ (ps: list PID) perm:
+   get_rx_gmap (update_ownership_batch σ ps perm) = get_rx_gmap σ.
     Proof.
       rewrite /get_rx_gmap.
       f_equal.
 Qed.
-      Lemma update_page_table_batch_preserve_rx σ (ps: list PID) perm:
-       (get_rx_agree (update_page_table_batch σ ps perm), get_rx_gmap (update_page_table_batch σ ps perm) ) =
+      Lemma update_ownership_batch_preserve_rx σ (ps: list PID) perm:
+       (get_rx_agree (update_ownership_batch σ ps perm), get_rx_gmap (update_ownership_batch σ ps perm) ) =
                                                (get_rx_agree σ, get_rx_gmap σ).
   Proof.
-    by rewrite update_page_table_batch_preserve_rx1 update_page_table_batch_preserve_rx2 .
+    by rewrite update_ownership_batch_preserve_rx1 update_ownership_batch_preserve_rx2 .
   Qed.
 
-   Lemma update_page_table_batch_preserve_trans σ (ps: list PID) perm:
-   get_trans_gmap (update_page_table_batch σ ps perm) = get_trans_gmap σ.
+   Lemma update_ownership_batch_preserve_trans σ (ps: list PID) perm:
+   get_trans_gmap (update_ownership_batch σ ps perm) = get_trans_gmap σ.
     Proof.
       rewrite /get_trans_gmap.
       f_equal.
 Qed.
-   Lemma update_page_table_batch_preserve_hpool σ (ps: list PID) perm:
-   get_hpool_gset (update_page_table_batch σ ps perm) = get_hpool_gset σ.
+   Lemma update_ownership_batch_preserve_hpool σ (ps: list PID) perm:
+   get_hpool_gset (update_ownership_batch σ ps perm) = get_hpool_gset σ.
     Proof.
       rewrite /get_hpool_gset.
       f_equal.
 Qed.
-   Lemma update_page_table_batch_preserve_receivers σ (ps: list PID) perm:
-   get_receivers_gmap (update_page_table_batch σ ps perm) = get_receivers_gmap σ.
+   Lemma update_ownership_batch_preserve_receivers σ (ps: list PID) perm:
+   get_receivers_gmap (update_ownership_batch σ ps perm) = get_receivers_gmap σ.
     Proof.
       rewrite /get_receivers_gmap.
       f_equal.
 Qed.
 
-    Lemma update_page_table_batch_preserve_other_page_tables σ ps perm i:
+    Lemma update_ownership_batch_preserve_other_page_tables σ ps perm i:
      i ≠ (get_current_vm σ) ->
-    (get_page_tables (update_page_table_batch σ ps perm)) !!! i =
+    (get_page_tables (update_ownership_batch σ ps perm)) !!! i =
     (get_page_tables σ) !!! i.
       Proof.
         intros.
-        rewrite /get_page_tables /update_page_table_batch /update_page_table_global_batch /=.
+        rewrite /get_page_tables /update_ownership_batch /update_ownership_global_batch /=.
+       rewrite vlookup_insert_ne.
+       rewrite /get_page_tables //.
+       done.
+       Qed.
+
+
+
+  Lemma update_access_batch_preserve_current_vm σ (ps: list PID) perm:
+   get_current_vm (update_access_batch σ ps perm) = get_current_vm σ.
+    Proof.
+      rewrite /get_current_vm.
+      f_equal.
+Qed.
+
+  Lemma update_access_batch_preserve_regs σ (ps: list PID) perm:
+   get_reg_gmap (update_access_batch σ ps perm) = get_reg_gmap σ.
+    Proof.
+      rewrite /get_reg_gmap.
+      f_equal.
+Qed.
+   Lemma update_access_batch_preserve_mem σ (ps: list PID) perm:
+   get_mem (update_access_batch σ ps perm) = get_mem σ.
+    Proof.
+      rewrite /get_mem.
+      f_equal.
+Qed.
+   Lemma update_access_batch_preserve_tx σ (ps: list PID) perm:
+   get_tx_agree (update_access_batch σ ps perm) = get_tx_agree σ.
+    Proof.
+      rewrite /get_tx_agree.
+      f_equal.
+Qed.
+       Lemma update_access_batch_preserve_rx1 σ (ps: list PID) perm:
+   get_rx_agree (update_access_batch σ ps perm) = get_rx_agree σ.
+    Proof.
+      rewrite /get_rx_agree.
+      f_equal.
+Qed.
+   Lemma update_access_batch_preserve_rx2 σ (ps: list PID) perm:
+   get_rx_gmap (update_access_batch σ ps perm) = get_rx_gmap σ.
+    Proof.
+      rewrite /get_rx_gmap.
+      f_equal.
+Qed.
+      Lemma update_access_batch_preserve_rx σ (ps: list PID) perm:
+       (get_rx_agree (update_access_batch σ ps perm), get_rx_gmap (update_access_batch σ ps perm) ) =
+                                               (get_rx_agree σ, get_rx_gmap σ).
+  Proof.
+    by rewrite update_access_batch_preserve_rx1 update_access_batch_preserve_rx2 .
+  Qed.
+
+   Lemma update_access_batch_preserve_trans σ (ps: list PID) perm:
+   get_trans_gmap (update_access_batch σ ps perm) = get_trans_gmap σ.
+    Proof.
+      rewrite /get_trans_gmap.
+      f_equal.
+Qed.
+   Lemma update_access_batch_preserve_hpool σ (ps: list PID) perm:
+   get_hpool_gset (update_access_batch σ ps perm) = get_hpool_gset σ.
+    Proof.
+      rewrite /get_hpool_gset.
+      f_equal.
+Qed.
+   Lemma update_access_batch_preserve_receivers σ (ps: list PID) perm:
+   get_receivers_gmap (update_access_batch σ ps perm) = get_receivers_gmap σ.
+    Proof.
+      rewrite /get_receivers_gmap.
+      f_equal.
+Qed.
+
+    Lemma update_access_batch_preserve_other_page_tables σ ps perm i:
+     i ≠ (get_current_vm σ) ->
+    (get_page_tables (update_access_batch σ ps perm)) !!! i =
+    (get_page_tables σ) !!! i.
+      Proof.
+        intros.
+        rewrite /get_page_tables /update_access_batch /update_access_global_batch /=.
        rewrite vlookup_insert_ne.
        rewrite /get_page_tables //.
        done.
@@ -690,7 +767,7 @@ Qed.
       Lemma get_access_gmap_is_accessible_true {σ i sacc} p:
             (get_access_gmap σ) !! i = Some (DfracOwn 1, to_agree (GSet sacc))->
             (p ∈ sacc <->
-            ∃ perm, (get_vm_page_table σ i) !! p =Some perm ∧ is_accessible perm = true).
+            ∃ perm, (get_vm_page_table σ i).2 !! p =Some perm ∧ is_accessible perm = true).
         Proof.
           intros.
           rewrite /get_access_gmap in H.
@@ -722,11 +799,11 @@ Qed.
             done.
         Qed.
 
-    Lemma update_page_table_batch_update_access_noaccess{ σ i sacc} {sps:gset PID} (ps: list PID) o :
+    Lemma update_access_batch_noaccess{ σ i sacc} {sps:gset PID} (ps: list PID):
      sps = (list_to_set ps)->
      i = (get_current_vm σ) ->
      (get_access_gmap σ) !! i = Some (DfracOwn 1, to_agree (GSet sacc)) ->
-     get_access_gmap (update_page_table_batch σ ps (o,NoAccess)) =
+     get_access_gmap (update_access_batch σ ps NoAccess) =
      <[(get_current_vm σ):= (DfracOwn 1, to_agree (GSet (sacc ∖ sps ) ))]>(get_access_gmap σ).
       Proof.
         intros.
@@ -755,7 +832,8 @@ Qed.
               apply map_filter_lookup_Some in H3.
               destruct H3.
               simplify_eq /=.
-              rewrite /get_vm_page_table /get_page_tables /update_page_table_batch /update_page_table_global_batch //= in H3.
+              rewrite /get_vm_page_table /get_page_tables /update_access_batch
+                      /update_access_global_batch //= in H3.
               rewrite vlookup_insert in H3.
               apply elem_of_difference.
               induction ps; simpl in *.
@@ -772,7 +850,8 @@ Qed.
                    rewrite /is_accessible //=.
                  }
                  rewrite not_elem_of_union.
-                 assert (Himp : x0.1 ∈ sacc ∧ x0.1 ∉ ((list_to_set ps):gset PID) ->(x0.1 ∈ sacc ∧ (x0.1 ∉ ({[a]}:gset PID)) ∧ x0.1 ∉ ((list_to_set ps):gset PID))).
+                 assert (Himp : x0.1 ∈ sacc ∧ x0.1 ∉ ((list_to_set ps):gset PID)
+                  ->(x0.1 ∈ sacc ∧ (x0.1 ∉ ({[a]}:gset PID)) ∧ x0.1 ∉ ((list_to_set ps):gset PID))).
                  { intros. destruct H; split;eauto. split. set_solver. done. }
                  apply Himp.
                  apply IHps;eauto.
@@ -789,7 +868,8 @@ Qed.
               apply elem_of_list_In .
               apply  elem_of_map_to_list.
               apply map_filter_lookup_Some.
-              rewrite /get_vm_page_table /get_page_tables /update_page_table_batch /update_page_table_global_batch /=.
+              rewrite /get_vm_page_table /get_page_tables /update_access_batch
+                      /update_access_global_batch /=.
               rewrite -H0 vlookup_insert.
               destruct H1;split;eauto.
               generalize dependent sps.
@@ -817,7 +897,8 @@ Qed.
                apply (elem_of_map_to_list' _ x0) in H3.
                apply map_filter_lookup_Some in H3.
                destruct H3.
-               rewrite /get_vm_page_table /get_page_tables /update_page_table_batch /update_page_table_global_batch //= in H2.
+               rewrite /get_vm_page_table /get_page_tables /update_access_batch
+                       /update_access_global_batch //= in H2.
                rewrite -H0 vlookup_insert in H2.
                apply elem_of_difference.
                generalize dependent sps.
@@ -838,7 +919,8 @@ Qed.
                  }
                  rewrite H.
                  rewrite not_elem_of_union.
-                 assert (Himp : x0.1 ∈ sacc ∧ x0.1 ∉ ((list_to_set ps):gset PID) ->(x0.1 ∈ sacc ∧ (x0.1 ∉ ({[a]}:gset PID)) ∧ x0.1 ∉ ((list_to_set ps):gset PID))).
+                 assert (Himp : x0.1 ∈ sacc ∧ x0.1 ∉ ((list_to_set ps):gset PID)
+                  ->(x0.1 ∈ sacc ∧ (x0.1 ∉ ({[a]}:gset PID)) ∧ x0.1 ∉ ((list_to_set ps):gset PID))).
                  {  intros. destruct H4; split;eauto. split. set_solver. done. }
                  apply Himp.
                  apply IHps;eauto.
@@ -855,7 +937,8 @@ Qed.
                  apply elem_of_list_In .
                  apply  elem_of_map_to_list.
                  apply map_filter_lookup_Some.
-                 rewrite /get_vm_page_table /get_page_tables /update_page_table_batch /update_page_table_global_batch /=.
+                 rewrite /get_vm_page_table /get_page_tables /update_access_batch
+                         /update_access_global_batch /=.
                  rewrite -H0 vlookup_insert.
                  destruct H1;split;eauto.
                  generalize dependent sps.
@@ -871,15 +954,13 @@ Qed.
                  set_solver.
         - rewrite (lookup_insert_ne _ i i0 _);eauto.
           set (l:= (map
-                      (λ v : VMID,
-                             (v,
-                              (DfracOwn 1,
-                               to_agree
-                                 (GSet
-                                    (list_to_set
-                                       (map (λ p : PID * permission, p.1)
-                                            (map_to_list
-                                               (filter (λ p : PID * permission, is_accessible p.2 = true) (get_vm_page_table σ v)))))))))
+              (λ v : VMID,
+              (v, (DfracOwn 1,
+                   to_agree (GSet
+                               (list_to_set
+                                  (map (λ p : PID * access, p.1)
+                      (map_to_list
+            (filter (λ p : PID * access, is_accessible p.2 = true) (get_vm_page_table σ v).2))))))))
                       list_of_vmids)) in *.
           destruct (list_to_map l !! i0) eqn:Heqn.
           + apply (elem_of_list_to_map_2 l i0 c) in Heqn.
@@ -892,12 +973,12 @@ Qed.
                inv_map_in.
                inversion H.
                do 7 f_equal.
-               rewrite /get_vm_page_table update_page_table_batch_preserve_other_page_tables //.
+               rewrite /get_vm_page_table update_access_batch_preserve_other_page_tables //.
             * inv_map_in.
               exists i0.
               split;eauto.
               do 8 f_equal.
-              rewrite /get_vm_page_table update_page_table_batch_preserve_other_page_tables //.
+              rewrite /get_vm_page_table update_access_batch_preserve_other_page_tables //.
           + apply (@not_elem_of_list_to_map_2 VMID (gmap VMID) _ _ _ _ _ _ _ _ gmap_finmap) in Heqn.
             apply (@not_elem_of_list_to_map_1 VMID (gmap VMID) _ _ _ _ _ _ _ _ gmap_finmap).
             intro P.
@@ -918,7 +999,7 @@ Qed.
             split;eauto.
             rewrite -H3.
             do 8 f_equal.
-            rewrite /get_vm_page_table update_page_table_batch_preserve_other_page_tables //.
+            rewrite /get_vm_page_table update_access_batch_preserve_other_page_tables //.
             destruct x.
             simpl in H2;inversion H3.
             by subst.
@@ -927,7 +1008,7 @@ Qed.
       Lemma get_owned_gmap_is_owned_true {σ i sown} p:
             (get_owned_gmap σ) !! i = Some (DfracOwn 1, to_agree (GSet sown))->
             (p ∈ sown <->
-            ∃ perm, (get_vm_page_table σ i) !! p =Some perm ∧ is_owned perm = true).
+            ∃ perm, (get_vm_page_table σ i).1 !! p =Some perm ∧ is_owned perm = true).
         Proof.
           intros.
           rewrite /get_owned_gmap in H.
@@ -960,11 +1041,11 @@ Qed.
         Qed.
 
 
-    Lemma update_page_table_batch_update_own_owned{ σ i sown} {sps:gset PID} (ps: list PID) a :
+    Lemma update_page_table_batch_update_own_owned{ σ i sown} {sps:gset PID} (ps: list PID):
      sps = (list_to_set ps)->
      i = (get_current_vm σ) ->
      (get_owned_gmap σ) !! i = Some (DfracOwn 1, to_agree (GSet sown)) ->
-     get_owned_gmap (update_page_table_batch σ ps (Owned,a)) =
+     get_owned_gmap (update_ownership_batch σ ps Owned) =
      <[i:= (DfracOwn 1, to_agree (GSet (sown ∪ sps ) ))]>(get_owned_gmap σ).
       Proof.
         intros.
@@ -992,7 +1073,8 @@ Qed.
               apply map_filter_lookup_Some in H3.
               destruct H3.
               simplify_eq /=.
-              rewrite /get_vm_page_table /get_page_tables /update_page_table_batch /update_page_table_global_batch //= in H3.
+              rewrite /get_vm_page_table /get_page_tables /update_ownership_batch
+                      /update_ownership_global_batch //= in H3.
               rewrite vlookup_insert in H3.
               apply elem_of_union.
               induction ps; simpl in *.
@@ -1000,10 +1082,10 @@ Qed.
                  apply (get_owned_gmap_is_owned_true x0.1 H1).
                  exists (x0.2).
                  split;eauto.
-              -- destruct (decide (a0=x0.1)).
+              -- destruct (decide (a=x0.1)).
                  right;set_solver.
                  assert (Himp :(x0.1 ∈ sown ∨ x0.1 ∈ ((list_to_set ps):gset PID))
-                                ->(x0.1 ∈ sown ∨ x0.1 ∈ {[a0]} ∪ ((list_to_set ps):gset PID))).
+                                ->(x0.1 ∈ sown ∨ x0.1 ∈ {[a]} ∪ ((list_to_set ps):gset PID))).
                  { intros. destruct H. left;done. right; set_solver. }
                  apply Himp.
                  apply IHps;eauto.
@@ -1020,145 +1102,177 @@ Qed.
               apply elem_of_list_In .
               apply elem_of_map_to_list.
               apply map_filter_lookup_Some.
-              rewrite /get_vm_page_table /get_page_tables /update_page_table_batch /update_page_table_global_batch /=.
+              rewrite /get_vm_page_table /get_page_tables /update_ownership_batch
+                      /update_ownership_global_batch /=.
               rewrite -H0 vlookup_insert.
               destruct H1;split;eauto.
               generalize dependent sps.
-              induction ps;simpl.
+              induction ps;simpl in *.
               done.
               intros.
-              (* rewrite H //= in H3. *)
-              destruct (decide (x=a0)).
-              subst a0.
+              destruct (decide (x=a)).
+              subst a.
               rewrite lookup_insert.
-              Admitted.
-              (* TODO: this lemma is not provable if we update ownership and accessiblity at the same time *)
-      (*         assert (Hneq: a ≠ x). *)
-      (*         { set_solver. } *)
-      (*         rewrite lookup_insert_ne;eauto. *)
-      (*         apply (IHps (list_to_set ps));eauto. *)
-      (*         set_solver. *)
-      (*     + inv_map_in. *)
-      (*       exists i. *)
-      (*       split;[|apply in_list_of_vmids]. *)
-      (*       do 4 f_equal. *)
-      (*       apply set_eq. *)
-      (*       intro. *)
-      (*       rewrite  elem_of_list_to_set. *)
-      (*       split. *)
-      (*       -- intros. *)
-      (*          inv_map_in. *)
-      (*          subst x. *)
-      (*          apply elem_of_list_In in H3. *)
-      (*          apply (elem_of_map_to_list' _ x0) in H3. *)
-      (*          apply map_filter_lookup_Some in H3. *)
-      (*          destruct H3. *)
-      (*          rewrite /get_vm_page_table /get_page_tables /update_page_table_batch /update_page_table_global_batch //= in H2. *)
-      (*          rewrite -H0 vlookup_insert in H2. *)
-      (*          apply elem_of_difference. *)
-      (*          generalize dependent sps. *)
-      (*          induction ps; simpl in *. *)
-      (*          ++ intros. *)
-      (*            split;[|set_solver]. *)
-      (*            apply (get_access_gmap_is_accessible_true x0.1 H1). *)
-      (*            exists x0.2. *)
-      (*            split;eauto. *)
-      (*          ++ intros. *)
-      (*            assert (Hneq: a ≠ x0.1). *)
-      (*            { destruct (decide (a=x0.1));eauto. *)
-      (*              subst a. *)
-      (*              rewrite lookup_insert in H2. *)
-      (*              inversion H2. *)
-      (*              rewrite -H5 in H3. *)
-      (*              rewrite /is_accessible //=. *)
-      (*            } *)
-      (*            rewrite H. *)
-      (*            rewrite not_elem_of_union. *)
-      (*            assert (Himp : x0.1 ∈ sacc ∧ x0.1 ∉ ((list_to_set ps):gset PID) ->(x0.1 ∈ sacc ∧ (x0.1 ∉ ({[a]}:gset PID)) ∧ x0.1 ∉ ((list_to_set ps):gset PID))). *)
-      (*            {  intros. destruct H4; split;eauto. split. set_solver. done. } *)
-      (*            apply Himp. *)
-      (*            apply IHps;eauto. *)
-      (*            rewrite lookup_insert_ne //= in H2. *)
-      (*       -- intros. *)
-      (*          apply elem_of_difference in H2. *)
-      (*          destruct H2. *)
-      (*          apply (get_access_gmap_is_accessible_true x H1) in H2;eauto. *)
-      (*          destruct H2. *)
-      (*          destruct H2. *)
-      (*          inv_map_in. *)
-      (*          exists (x,x0). *)
-      (*          split;eauto. *)
-      (*            apply elem_of_list_In . *)
-      (*            apply  elem_of_map_to_list. *)
-      (*            apply map_filter_lookup_Some. *)
-      (*            rewrite /get_vm_page_table /get_page_tables /update_page_table_batch /update_page_table_global_batch /=. *)
-      (*            rewrite -H0 vlookup_insert. *)
-      (*            destruct H1;split;eauto. *)
-      (*            generalize dependent sps. *)
-      (*            induction ps;simpl. *)
-      (*            done. *)
-      (*            intros. *)
-      (*            rewrite H in H3. *)
-      (*            simpl in H3. *)
-      (*            assert (Hneq: a ≠ x). *)
-      (*            { set_solver. } *)
-      (*            rewrite lookup_insert_ne;eauto. *)
-      (*            apply (IHps (list_to_set ps));eauto. *)
-      (*            set_solver. *)
-      (*   - rewrite (lookup_insert_ne _ i i0 _);eauto. *)
-      (*     set (l:= (map *)
-      (*                 (λ v : VMID, *)
-      (*                        (v, *)
-      (*                         (DfracOwn 1, *)
-      (*                          to_agree *)
-      (*                            (GSet *)
-      (*                               (list_to_set *)
-      (*                                  (map (λ p : PID * permission, p.1) *)
-      (*                                       (map_to_list *)
-      (*                                          (filter (λ p : PID * permission, is_accessible p.2 = true) (get_vm_page_table σ v))))))))) *)
-      (*                 list_of_vmids)) in *. *)
-      (*     destruct (list_to_map l !! i0) eqn:Heqn. *)
-      (*     + apply (elem_of_list_to_map_2 l i0 c) in Heqn. *)
-      (*       apply elem_of_list_In in Heqn. *)
-      (*       apply in_map_iff in Heqn. *)
-      (*       inversion Heqn;clear Heqn. *)
-      (*       destruct H2 as [H3 HIn];inversion H3;subst;clear H3. *)
-      (*       apply (@elem_of_list_to_map_1' VMID (gmap VMID) _ _ _ _ _ _ _ _ gmap_finmap). *)
-      (*       *  intros. *)
-      (*          inv_map_in. *)
-      (*          inversion H. *)
-      (*          do 7 f_equal. *)
-      (*          rewrite /get_vm_page_table update_page_table_batch_preserve_other_page_tables //. *)
-      (*       * inv_map_in. *)
-      (*         exists i0. *)
-      (*         split;eauto. *)
-      (*         do 8 f_equal. *)
-      (*         rewrite /get_vm_page_table update_page_table_batch_preserve_other_page_tables //. *)
-      (*     + apply (@not_elem_of_list_to_map_2 VMID (gmap VMID) _ _ _ _ _ _ _ _ gmap_finmap) in Heqn. *)
-      (*       apply (@not_elem_of_list_to_map_1 VMID (gmap VMID) _ _ _ _ _ _ _ _ gmap_finmap). *)
-      (*       intro P. *)
-      (*       apply Heqn. *)
-      (*       apply elem_of_list_In. *)
-      (*       apply in_map_iff. *)
-      (*       apply elem_of_list_In in P. *)
-      (*       apply in_map_iff in P. *)
-      (*       destruct P. *)
-      (*       exists x. *)
-      (*       destruct H2. *)
-      (*       split;eauto. *)
-      (*       apply in_map_iff. *)
-      (*       apply in_map_iff in H3. *)
-      (*       destruct H3. *)
-      (*       exists x0. *)
-      (*       destruct H3. *)
-      (*       split;eauto. *)
-      (*       rewrite -H3. *)
-      (*       do 8 f_equal. *)
-      (*       rewrite /get_vm_page_table update_page_table_batch_preserve_other_page_tables //. *)
-      (*       destruct x. *)
-      (*       simpl in H2;inversion H3. *)
-      (*       by subst. *)
-      (* Qed. *)
+              rewrite /is_owned in H3.
+              destruct x0;eauto.
+              done.
+              rewrite lookup_insert_ne;eauto.
+              inv_map_in.
+              exists (x,Owned).
+              split;eauto.
+              apply elem_of_list_In .
+              apply elem_of_map_to_list.
+              apply map_filter_lookup_Some.
+              rewrite /get_vm_page_table /get_page_tables /update_ownership_batch
+                      /update_ownership_global_batch /=.
+              split;eauto.
+              rewrite -H0 vlookup_insert //=.
+              generalize dependent sps.
+              induction ps;simpl in *.
+              intros.
+              set_solver.
+              intros.
+              destruct (decide (x=a)).
+              subst a.
+              rewrite lookup_insert //.
+              rewrite lookup_insert_ne;eauto.
+              apply (IHps (list_to_set ps));eauto.
+              set_solver.
+          + inv_map_in.
+            exists i.
+            split;[|apply in_list_of_vmids].
+            do 4 f_equal.
+            apply set_eq.
+            intro.
+            rewrite  elem_of_list_to_set.
+            split.
+            -- intros.
+               inv_map_in.
+               subst x.
+               apply elem_of_list_In in H3.
+               apply (elem_of_map_to_list' _ x0) in H3.
+               apply map_filter_lookup_Some in H3.
+               destruct H3.
+               rewrite /get_vm_page_table /get_page_tables /update_ownership_batch
+                       /update_ownership_global_batch //= in H2.
+               rewrite -H0 vlookup_insert in H2.
+               apply elem_of_union.
+               generalize dependent sps.
+               induction ps; simpl in *.
+               ++ left.
+                 apply (get_owned_gmap_is_owned_true x0.1 H1).
+                 exists (x0.2).
+                 split;eauto.
+              ++ intros.
+                destruct (decide (a=x0.1)).
+                 right;set_solver.
+                 rewrite H.
+                 assert (Himp :(x0.1 ∈ sown ∨ x0.1 ∈ ((list_to_set ps):gset PID))
+                                ->(x0.1 ∈ sown ∨ x0.1 ∈ {[a]} ∪ ((list_to_set ps):gset PID))).
+                 { intros. destruct H4. left;done. right; set_solver. }
+                 apply Himp.
+                 apply IHps;eauto.
+                 rewrite lookup_insert_ne in H2;done.
+            -- intros.
+               apply elem_of_union in H2.
+               destruct H2.
+               apply (get_owned_gmap_is_owned_true x H1) in H2;eauto.
+               destruct H2.
+               destruct H2.
+               inv_map_in.
+               exists (x,x0).
+               split;eauto.
+               apply elem_of_list_In .
+               apply  elem_of_map_to_list.
+               apply map_filter_lookup_Some.
+               rewrite /get_vm_page_table /get_page_tables /update_ownership_batch
+                       /update_ownership_global_batch /=.
+               rewrite -H0 vlookup_insert.
+               destruct H1;split;eauto.
+               generalize dependent sps.
+               induction ps;simpl in *;intros.
+               done.
+               intros.
+               destruct (decide (x=a)).
+              subst a.
+              rewrite lookup_insert.
+              rewrite /is_owned in H3.
+              destruct x0;eauto.
+              done.
+              rewrite lookup_insert_ne;eauto.
+              inv_map_in.
+              exists (x,Owned).
+              split;eauto.
+              apply elem_of_list_In .
+              apply elem_of_map_to_list.
+              apply map_filter_lookup_Some.
+              rewrite /get_vm_page_table /get_page_tables /update_ownership_batch
+                      /update_ownership_global_batch /=.
+              split;eauto.
+              rewrite -H0 vlookup_insert //=.
+              generalize dependent sps.
+              induction ps;simpl in *.
+              intros.
+              set_solver.
+              intros.
+              destruct (decide (x=a)).
+              subst a.
+              rewrite lookup_insert //.
+              rewrite lookup_insert_ne;eauto.
+              apply (IHps (list_to_set ps));eauto.
+              set_solver.
+        - rewrite (lookup_insert_ne _ i i0 _);eauto.
+          set (l:= (map
+                      (λ v : VMID,
+                             (v, (DfracOwn 1,
+                               to_agree (GSet
+                                    (list_to_set
+                                       (map (λ p : PID * ownership, p.1)
+                                            (map_to_list
+                (filter (λ p : PID * ownership, is_owned p.2 = true) (get_vm_page_table σ v).1))))))))
+                      list_of_vmids)) in *.
+          destruct (list_to_map l !! i0) eqn:Heqn.
+          + apply (elem_of_list_to_map_2 l i0 c) in Heqn.
+            apply elem_of_list_In in Heqn.
+            apply in_map_iff in Heqn.
+            inversion Heqn;clear Heqn.
+            destruct H2 as [H3 HIn];inversion H3;subst;clear H3.
+            apply (@elem_of_list_to_map_1' VMID (gmap VMID) _ _ _ _ _ _ _ _ gmap_finmap).
+            *  intros.
+               inv_map_in.
+               inversion H.
+               do 7 f_equal.
+               rewrite /get_vm_page_table update_ownership_batch_preserve_other_page_tables //.
+            * inv_map_in.
+              exists i0.
+              split;eauto.
+              do 8 f_equal.
+              rewrite /get_vm_page_table update_ownership_batch_preserve_other_page_tables //.
+          + apply (@not_elem_of_list_to_map_2 VMID (gmap VMID) _ _ _ _ _ _ _ _ gmap_finmap) in Heqn.
+            apply (@not_elem_of_list_to_map_1 VMID (gmap VMID) _ _ _ _ _ _ _ _ gmap_finmap).
+            intro P.
+            apply Heqn.
+            apply elem_of_list_In.
+            apply in_map_iff.
+            apply elem_of_list_In in P.
+            apply in_map_iff in P.
+            destruct P.
+            exists x.
+            destruct H2.
+            split;eauto.
+            apply in_map_iff.
+            apply in_map_iff in H3.
+            destruct H3.
+            exists x0.
+            destruct H3.
+            split;eauto.
+            rewrite -H3.
+            do 8 f_equal.
+            rewrite /get_vm_page_table update_ownership_batch_preserve_other_page_tables //.
+            destruct x.
+            simpl in H2;inversion H3.
+            by subst.
+      Qed.
 
   Lemma insert_transaction_preserve_current_vm σ h trans:
    get_current_vm (insert_transaction σ h trans) = get_current_vm σ.
